Veritas.SeqMachine.fst
@@ -16,9 +16,11 @@ let lemma_valid_prefix (sm: seq_machine) (s: (seq (elem_type sm)){valid sm s}) (
     lemma_reduce_identity (fail_state sm) (trans_fn sm) (suffix s (length s - i))
   )
 
-let lemma_notempty_implies_noninit (sm: seq_machine) (s: seq (elem_type sm){length s > 0}):
-  Lemma (init_state sm <> seq_machine_run sm s) = 
+let lemma_notempty_implies_noninit (sm: seq_machine) (s: seq (elem_type sm)):
+  Lemma (length s > 0 ==> init_state sm <> seq_machine_run sm s) = 
   let n = length s in
+  if n = 0 then ()
+  else
   let s1 = seq_machine_run sm (prefix s 1) in  
   lemma_reduce_prefix (init_state sm) (trans_fn sm) s 1;
   lemma_reduce_singleton (init_state sm) (trans_fn sm) (prefix s 1);
