Veritas.Verifier.CorrectDefs.fst
@@ -49,7 +49,7 @@ let t_verifiable (il: tid_vlog): bool =
 type t_verifiable_log = il: tid_vlog {t_verifiable il}
 
 (* Full collection of verifier logs one per thread *)
-type g_vlog = seq vlog
+type g_vlog = (gl:seq vlog{length gl > 0})
 
 (* a slightly different view of verifier log obtained by
  * attaching a tid (index) to each thread verifier log *)
@@ -195,151 +195,6 @@ let evict_value (il:t_verifiable_log) (i:nat{i < tv_length il /\
   | EvictB k _ -> stored_value sti k
   | EvictBM k _ _ -> stored_value sti k
 
-type its_log (n:nat) = 
-  s:seq (idx_elem #vlog_entry n){g_verifiable (partition_idx_seq s)}
-
-(* the prefix of an its log *)
-let its_prefix (#n:nat) (itsl: its_log n) (i:nat{i <= length itsl}): 
-  (itsl':its_log n{length itsl' = i}) =
-  let itsl': seq (idx_elem #vlog_entry n) = prefix itsl i in
-  let gl = partition_idx_seq itsl in
-  let idgl = g_tid_vlog gl in
-  
-  let gl' = partition_idx_seq itsl' in
-  let idgl' = g_tid_vlog gl' in
-
-  let aux (id:nat{id < n}):
-    Lemma (requires True)
-          (ensures (t_verifiable (index idgl' id)))
-          [SMTPat (t_verifiable (index idgl' id))]    
-    = 
-    let (_,l') = index idgl' id in
-    //let (_,l) = index idgl id in    
-    lemma_partition_idx_prefix_comm itsl i  id;
-    lemma_verifiable_implies_prefix_verifiable (index idgl id) (length l');
-    ()
-  in
-  itsl'
-
-
-(* extended time sequence log (with evict values) *)
-let rec time_seq_ext (#n:nat) (itsl: its_log n):
-  Tot (le:vlog_ext{project_seq itsl = to_vlog le})
-  (decreases (length itsl))
-  =
-  let m = length itsl in
-  if m = 0 then (
-    lemma_empty itsl;
-    lemma_empty (project_seq itsl);
-    let r = empty #vlog_entry_ext in
-    lemma_empty (to_vlog r);
-    r
-  )
-  else (
-    let (e,id) = telem itsl in
-
-    (* recurse *)
-    let itsl' = its_prefix itsl (m - 1) in
-    let r' = time_seq_ext itsl' in
-
-    (* project seq of itsl and itsl' differ by log entry e *)
-    lemma_unzip_extend itsl;
-    assert(project_seq itsl = append1 (project_seq itsl') e);
-
-    if is_evict e then (
-      (* log entries of verifier thread id *)
-      let gl = partition_idx_seq itsl in
-      let l = index gl id in
-      assert(snd (index (g_tid_vlog gl) id) = l);
-
-      (* since l is verifiable, the value at last position is well-defined *)
-      assert(t_verifiable (id, l));
-      (* prove length l > 0 *)
-      lemma_partition_idx_extend1 itsl;
-
-      let v = evict_value (id, l) (length l - 1) in
-
-      let r = append1 r' (Evict e v) in
-      lemma_prefix1_append r' (Evict e v);
-      lemma_map_extend to_vlog_entry r;
-      r
-    )
-    else (
-      let r = append1 r' (NEvict e) in
-      lemma_prefix1_append r' (NEvict e);
-      lemma_map_extend to_vlog_entry r;
-      r
-    )
-  )
-
-let lemma_its_prefix_ext (#n:nat) (itsl:its_log n) (i:nat{i <= length itsl}):
-  Lemma (requires True)
-        (ensures (time_seq_ext (its_prefix itsl i) = prefix (time_seq_ext itsl) i))
-        [SMTPat (time_seq_ext (its_prefix itsl i))] = 
-  admit()
-
-type eac_ts_log (n:nat) = itsl: its_log n {is_eac_log (time_seq_ext itsl)}
-type non_eac_ts_log (n:nat) = itsl: its_log n {not (is_eac_log (time_seq_ext itsl))}
-
-(* the eac state of a key after processing an eac_log *)
-(* TODO: remove this *)
-let eac_state_key (le: vlog_ext) (k:key): eac_state = 
-  let lek = partn eac_sm k le in
-  seq_machine_run eac_smk lek
-
-(* the eac state of a key at the end of an its log *)
-let eac_state_of_key (#n:nat) (itsl: its_log n) (k:key): eac_state = 
-  let tsle = time_seq_ext itsl in 
-  let tslek = partn eac_sm k tsle in
-  seq_machine_run eac_smk tslek
-
-(* is the eac state of key at the end of its_log init *)
-let is_eac_state_init (#n:nat) (itsl: its_log n) (k:key): bool =
-  eac_state_of_key itsl k = EACInit
-
-(* is the key k in evicted state in *)
-let is_eac_state_evicted (#n:nat) (itsl: its_log n) (k:key): bool = 
-  EACEvicted? (eac_state_of_key itsl k)
-
-(* is the key currently evicted into merkle *)
-let is_eac_state_evicted_merkle (#n:nat) (itsl: its_log n) (k:key): bool = 
-  let st = eac_state_of_key itsl k in
-  match st with
-  | EACEvicted m v -> m = MAdd 
-  | _ -> false
-
-(* is the key currently evicted into merkle *)
-let is_eac_state_evicted_blum (#n:nat) (itsl: its_log n) (k:key): bool = 
-  let st = eac_state_of_key itsl k in
-  match st with
-  | EACEvicted m v -> m = BAdd
-  | _ -> false
-
-(* is the key k in instore state after processing its_log *)
-let is_eac_state_instore (#n:nat) (itsl: its_log n) (k:key):bool = 
-  EACInStore? (eac_state_of_key itsl k)
-
-(* the state of a verifier thread after processing entries in a log *)
-let verifier_thread_state (#n:nat) (itsl: its_log n) (id:nat{id < n}): (st:vtls{Valid? st}) = 
-  let gl = partition_idx_seq itsl in
-  assert(t_verifiable (index (attach_index gl) id));
-  t_verify id (index gl id)
-
-(* 
- * when the eac state of a key is Init (no operations on the key yet) no 
- * thread contains the key in its store 
- *)
-let lemma_eac_state_init_store 
-   (#n:nat) 
-   (itsl: eac_ts_log n) (k: key{k <> Root && is_eac_state_init itsl k}) (id:nat{id < n}):
-   Lemma (not (store_contains (thread_store (verifier_thread_state itsl id)) k)) 
-   = admit()
-
-(* when the eac state of a key is EACEvicted then no thread contains the key in its store *)
-let lemma_eac_state_evicted_store (#n:nat) (itsl: eac_ts_log n) 
-  (k: key{is_eac_state_evicted itsl k}) (id:nat{id < n}):
-    Lemma (not (store_contains (thread_store (verifier_thread_state itsl id)) k)) = admit()
-
 (* does a log have some add entry *)
 let has_some_add (l:seq vlog_entry): bool = 
   exists_sat_elems is_add l
@@ -347,62 +202,14 @@ let has_some_add (l:seq vlog_entry): bool =
 (* does a log have some add of key k *)
 let has_some_add_of_key (k:key) (l:seq vlog_entry): bool = 
   exists_sat_elems (is_add_of_key k) l 
-  
-(* when the eac state of a key is "instore" then there is always a previous add *)
-let lemma_eac_state_instore_implies_prev_add (#n:nat) (itsl: eac_ts_log n) (k:key{is_eac_state_instore itsl k}):
-  Lemma (has_some_add_of_key k (project_seq itsl)) = admit()
 
-(* when the eac state of a key is instore return the index of the last add that transitioned
- * the key k to "instore" *)
-let last_add_idx (#n:nat) (itsl: eac_ts_log n) (k: key{is_eac_state_instore itsl k}): seq_index itsl =
-   lemma_eac_state_instore_implies_prev_add itsl k;
-   last_index (is_add_of_key k) (project_seq itsl)
-
-(* the verifier thread where the last add of key k happens *)
-let last_add_tid (#n:nat) (itsl: eac_ts_log n) (k: key{is_eac_state_instore itsl k}): (tid:nat{tid < n}) =
-  snd (index itsl (last_add_idx itsl k))
-
-(* if the eac_state of k is instore, then that k is in the store of the verifier thread of its last add *)
-let lemma_eac_state_instore (#n:nat) (itsl: eac_ts_log n) (k:key{is_eac_state_instore itsl k}):
-  Lemma (store_contains (thread_store (verifier_thread_state itsl (last_add_tid itsl k))) k) = admit()
-
-(* if the eac state of k is instore, then k is not in the store of any verifier thread other than 
- * its last add thread *)
-let lemma_eac_state_instore2 (#n:nat) (itsl: eac_ts_log n) (k:key{is_eac_state_instore itsl k}) (id:nat{id < n}):
-  Lemma (requires (id <> last_add_tid itsl k))
-        (ensures (not (store_contains (thread_store (verifier_thread_state itsl id)) k))) = admit()
-
-(* the root is always in thread 0 *)
-let lemma_root_in_store0 (#n:pos) (itsl: eac_ts_log n):
-  Lemma (store_contains (thread_store (verifier_thread_state itsl 0)) Root) = admit()
-
-let lemma_root_not_in_store (#n:pos) (itsl: eac_ts_log n) (tid:pos {tid < n}):
-  Lemma (not (store_contains (thread_store (verifier_thread_state itsl tid)) Root)) = admit()
-
-(* the evicted value is always of the correct type for the associated key *)
-let lemma_evict_value_correct_type (#n:pos) (itsl: eac_ts_log n) (k:key{is_eac_state_evicted itsl k}):
-  Lemma (is_value_of k (EACEvicted?.v (eac_state_of_key itsl k))) = admit()
-
-(* 
- * for keys in a thread store, return the value in the thread store; 
- * for other keys return the last evict value or null (init)
- *)
-let eac_value (#n:pos) (itsl: eac_ts_log n) (k:key): value_type_of k = 
-  if k = Root then (
-    lemma_root_in_store0 itsl;
-    stored_value (thread_store (verifier_thread_state itsl 0)) Root
-  )
-  else 
-    let es = eac_state_of_key itsl k in
-    match es with
-    | EACInit -> init_value k 
-    | EACEvicted _ v -> lemma_evict_value_correct_type itsl k; v
-    | EACInStore _ _ -> 
-      (* the store where the last add happened contains key k *)
-      let tid = last_add_tid itsl k in
-      let st = thread_store (verifier_thread_state itsl tid) in
-        
-      lemma_eac_state_instore itsl k;
-      assert(store_contains st k);
-
-      stored_value st k
+(* the thread id of a verifier remains unchanged *)
+let rec lemma_thread_id (il:t_verifiable_log):
+  Lemma (requires True)
+        (ensures (thread_id (t_verify (fst il) (snd il)) = (fst il)))
+        (decreases (tv_length il)) = 
+  let (id,l) = il in
+  let n = length l in
+  if n = 0 then ()
+  else
+    lemma_thread_id (id, hprefix l)
