Veritas.Verifier.EAC.fst
@@ -6,13 +6,18 @@ open Veritas.EAC
 open Veritas.Hash
 open Veritas.Interleave
 open Veritas.Key
+open Veritas.MultiSet
 open Veritas.MultiSetHash
 open Veritas.Record
 open Veritas.SeqAux
 open Veritas.SeqMachine
 open Veritas.State
 open Veritas.Verifier
+open Veritas.Verifier.Blum
 open Veritas.Verifier.CorrectDefs
+open Veritas.Verifier.TSLog
+
+module MH = Veritas.MultiSetHash
 
 (* generalized single- and multi-set hash collision *)
 type hash_collision_gen =
@@ -23,25 +28,30 @@ type hash_collision_gen =
 let hash_collision_contra (_:unit{False}): hash_collision_gen = 
   SingleHashCollision (Collision (DVal Null) (DVal Null))
 
+let max_eac_ts_prefix (#p:pos) (itsl: non_eac_ts_log p): eac_ts_log p =
+  let tsle = time_seq_ext itsl in
+  let i = max_eac_prefix tsle in
+  its_prefix itsl i
+
 (* the entry that causes the eac_invalidation *)
-let invalidating_log_entry (#n:nat) (itsl: non_eac_ts_log n): vlog_entry_ext = 
+let invalidating_log_entry (#n:pos) (itsl: non_eac_ts_log n): vlog_entry_ext = 
   let tsle = time_seq_ext itsl in  
   let i = max_eac_prefix tsle in  
   index tsle i
 
 (* the key that causes the eac_invalidation *)
-let eac_invalidating_key (#n:nat) (itsl: non_eac_ts_log n): key =
+let eac_invalidating_key (#n:pos) (itsl: non_eac_ts_log n): key =
   vlog_entry_ext_key (invalidating_log_entry itsl)
 
 (* last valid eac state *)
-let last_valid_eac_state (#n:nat) (itsl: non_eac_ts_log n): eac_state = 
+let last_valid_eac_state (#n:pos) (itsl: non_eac_ts_log n): eac_state = 
   let tsle = time_seq_ext itsl in  
   let i = max_eac_prefix tsle in
   let k = eac_invalidating_key itsl in
-  eac_state_key (prefix tsle i) k
+  eac_state_of_key (its_prefix itsl i) k
   
 (* applying the invalidating entry on the last valid state produces EAC failure *)
-let lemma_invalidation (#n:nat) (itsl: non_eac_ts_log n):
+let lemma_invalidation (#n:pos) (itsl: non_eac_ts_log n):
   Lemma (EACFail <> last_valid_eac_state itsl /\
          EACFail = eac_add (invalidating_log_entry itsl) (last_valid_eac_state itsl)) =            
   let tsl = project_seq itsl in
@@ -89,13 +99,13 @@ let lemma_invalidation (#n:nat) (itsl: non_eac_ts_log n):
 
   ()         
 
-let its_vlog_entry (#n:nat) (itsl: its_log n) (i:seq_index itsl): vlog_entry =
+let its_vlog_entry (#n:pos) (itsl: its_log n) (i:seq_index itsl): vlog_entry =
   fst (index itsl i)
 
-let its_thread_id (#n:nat) (itsl: its_log n) (i:seq_index itsl): (tid:nat{tid < n}) =
+let its_thread_id (#n:pos) (itsl: its_log n) (i:seq_index itsl): (tid:nat{tid < n}) =
   snd (index itsl i)
 
-let lemma_verifier_thread_state_extend (#n:nat) (itsl: its_log n{length itsl > 0}):
+let lemma_verifier_thread_state_extend (#n:pos) (itsl: its_log n{length itsl > 0}):
   Lemma (verifier_thread_state itsl (its_thread_id itsl (length itsl - 1)) == 
          t_verify_step (verifier_thread_state (its_prefix itsl (length itsl - 1)) 
                                               (its_thread_id itsl (length itsl - 1)))
@@ -108,18 +118,20 @@ let lemma_verifier_thread_state_extend (#n:nat) (itsl: its_log n{length itsl > 0
   lemma_partition_idx_extend1 itsl;
   lemma_prefix1_append (index gl' id) e
 
-let lemma_time_seq_ext_correct (#n:nat) (itsl: its_log n) (i:seq_index itsl):
+let lemma_time_seq_ext_correct (#n:pos) (itsl: its_log n) (i:seq_index itsl):
   Lemma (requires True)
         (ensures (its_vlog_entry itsl i = to_vlog_entry (index (time_seq_ext itsl) i))) 
         [SMTPat (to_vlog_entry (index (time_seq_ext itsl) i))] =
   lemma_unzip_index itsl i
 
 (* if an operation requires the key in store, it cannot be the first operation *)
-let lemma_non_eac_init_requires_key_in_store (#n:nat) 
+let lemma_non_eac_init_requires_key_in_store (#n:pos) 
   (itsl: non_eac_ts_log n{last_valid_eac_state itsl = EACInit /\
                            requires_key_in_store (to_vlog_entry (invalidating_log_entry itsl)) /\
                            Root <> vlog_entry_key (to_vlog_entry (invalidating_log_entry itsl))}):  
   hash_collision_gen = 
+  admit()
+  (*
   let tsle = time_seq_ext itsl in
   let i = max_eac_prefix tsle in
  
@@ -133,12 +145,15 @@ let lemma_non_eac_init_requires_key_in_store (#n:nat)
   let k = vlog_entry_key e in
   lemma_eac_state_init_store itsli k tid;
   hash_collision_contra ()
+  *)
 
 (* the first operation for a key cannot be evict *)
-let lemma_non_eac_init_evict (#n:nat)
+let lemma_non_eac_init_evict (#n:pos)
   (itsl: non_eac_ts_log n{last_valid_eac_state itsl = EACInit /\
                            requires_key_in_store (to_vlog_entry (invalidating_log_entry itsl)) /\
                            is_evict (to_vlog_entry (invalidating_log_entry itsl))}): hash_collision_gen =
+  admit()
+  (*
   let tsle = time_seq_ext itsl in
   let i = max_eac_prefix tsle in
  
@@ -153,14 +168,51 @@ let lemma_non_eac_init_evict (#n:nat)
   lemma_root_never_evicted (verifier_thread_state itsli tid) e;  
   assert(k <> Root);                               
   lemma_non_eac_init_requires_key_in_store itsl
+  *)
 
 (* the first operation for a key cannot be a blum add *)
 let lemma_non_eac_init_addb (#n)
   (itsl: non_eac_ts_log n{last_valid_eac_state itsl = EACInit /\
                            AddB? (to_vlog_entry (invalidating_log_entry itsl))}): hash_collision_gen =
-  admit()                           
+  let tsle = time_seq_ext itsl in
+  let i = max_eac_prefix tsle in
+  let (e,tid) = index itsl i in
+  let k = vlog_entry_key e in
 
-let lemma_non_eac_time_seq_implies_hash_collision (#n:nat) (itsl: non_eac_ts_log n): hash_collision_gen = 
+  (* the i'th entry is a blum add *)
+  assert(is_blum_add (index itsl i));
+  let be = blum_add_elem (index itsl i) in
+
+  
+  assert(to_vlog_entry (index tsle i) = e);
+  let itsli = its_prefix itsl i in
+  let tslei = time_seq_ext itsli in
+  assert(tslei = prefix tsle i);
+  let tsleik = partn eac_sm k tslei in
+  
+  lemma_notempty_implies_noninit eac_smk tsleik;
+  assert(length tsleik = 0);
+
+
+
+
+  if contains be (ts_evict_set itsl) then (
+    (* the evict that corresponds to blum add happens before i *)
+    let j = index_blum_evict itsl be in
+    lemma_evict_before_add itsl i;
+    assert(j < i);
+
+    assert(blum_evict_elem itsl j = be);
+    assert(MH.key_of be = key_of itsl j);        
+    assert(k = key_of itsl j);
+
+    admit()                           
+  )
+  else
+  
+    admit()
+
+let lemma_non_eac_time_seq_implies_hash_collision (#n:pos) (itsl: non_eac_ts_log n): hash_collision_gen = 
   let st = last_valid_eac_state itsl in
   let ee = invalidating_log_entry itsl in
   match st with
