Veritas.Verifier.Blum.fsti
@@ -1,0 +1,107 @@
+module Veritas.Verifier.Blum
+
+open FStar.Seq
+open Veritas.Interleave
+open Veritas.Key
+open Veritas.MultiSet
+open Veritas.MultiSetHash
+open Veritas.SeqAux
+open Veritas.Verifier
+open Veritas.Verifier.CorrectDefs
+open Veritas.Verifier.TSLog
+
+module M=Veritas.MultiSetHash
+module TL=Veritas.Verifier.TSLog
+
+(* global add sequence *)
+val g_add_seq (gl: g_verifiable_log): seq (ms_hashfn_dom)
+
+(* multiset derived from all the blum adds in gl *)
+let g_add_set (gl: g_verifiable_log): mset ms_hashfn_dom =
+  seq2mset (g_add_seq gl)
+
+(* the hadd that the verifier computes is the multiset hash of all the adds *)
+val lemma_g_hadd_correct (gl: g_verifiable_log):
+  Lemma (g_hadd gl = ms_hashfn (g_add_seq gl))
+
+(* a single sequence containing all the blum evicts *)
+val g_evict_seq (gl: g_verifiable_log): seq ms_hashfn_dom 
+
+let g_evict_set (gl: g_verifiable_log): mset ms_hashfn_dom = 
+  seq2mset (g_evict_seq gl)
+
+(* the global evict set is a set (not a multiset) *)
+val g_evict_set_is_set (gl: g_verifiable_log): 
+  Lemma (is_set (g_evict_set gl))
+
+val lemma_ghevict_correct (gl: g_verifiable_log):
+  Lemma (g_hevict gl = ms_hashfn (g_evict_seq gl))
+
+(* is the i'th index of itsl a blum add *)
+let is_blum_add (#p:nat) (ie:idx_elem #vlog_entry p):bool =
+  let (e,_) = ie in
+  match e with
+  | AddB _ _ _ -> true
+  | _ -> false
+
+(* get the blum add element from an index *)
+let blum_add_elem (#p:nat) (ie:idx_elem #vlog_entry p{is_blum_add ie}):
+  ms_hashfn_dom = 
+  let (e,_) = ie in
+  match e with
+  | AddB r t j -> MHDom r t j
+
+(* sequence of blum adds in the time sequenced log *)
+val ts_add_seq (#n:pos) (itsl: its_log n): seq ms_hashfn_dom
+
+(* the addset in a time sequenced log *)
+let ts_add_set (#n:pos) (itsl: its_log n): mset ms_hashfn_dom 
+  = seq2mset (ts_add_seq itsl)
+
+(* sequence of blum adds restricted to key k *)
+val ts_add_seq_key (#n:pos) (itsl: its_log n) (k:key): seq ms_hashfn_dom
+
+(* the addset restricted to key k *)
+let ts_add_set_key (#n:pos) (itsl: its_log n) (k:key): mset ms_hashfn_dom
+  = seq2mset (ts_add_seq_key itsl k)
+
+(* the blum adds in the time sequenced log should be the same as global add set *)
+val lemma_ts_add_set_correct (#n:pos) (itsl: its_log n): 
+  Lemma (ts_add_set itsl == g_add_set (partition_idx_seq itsl))
+
+(* is the index i of ts log an blum evict *)
+val is_blum_evict (#p:pos) (itsl: its_log p) (i: seq_index itsl): bool
+
+(* get the blum evict element from an index *)
+val blum_evict_elem (#p:pos) (itsl: its_log p) (i:seq_index itsl{is_blum_evict itsl i}):
+  (e:ms_hashfn_dom{M.key_of e = TL.key_of itsl i})
+
+(* sequence of evicts in time sequence log *)
+val ts_evict_seq (#n:pos) (itsl: its_log n): seq ms_hashfn_dom
+
+(* set of evicts in time sequence log *)
+let ts_evict_set (#n:pos) (itsl: its_log n): mset ms_hashfn_dom = 
+  seq2mset (ts_evict_seq itsl)
+
+(* the evict sequence restricted to key k *)
+val ts_evict_seq_key (#n:pos) (itsl: its_log n) (k:key): seq ms_hashfn_dom
+
+let ts_evict_set_key (#n:pos) (itsl: its_log n) (k:key): mset ms_hashfn_dom= 
+  seq2mset (ts_evict_seq_key itsl k)
+
+(* the blum evicts in time sequenced log should be the same as global evict set *)
+val lemma_ts_evict_set_correct (#n:pos) (itsl: its_log n):
+  Lemma (ts_evict_set itsl == g_evict_set (partition_idx_seq itsl))
+
+(* since evict_set is a pure set (not a multiset) we can identify the unique index 
+ * for each element of the set *)
+val index_blum_evict (#p:pos) (itsl: its_log p) (e: ms_hashfn_dom {contains e (ts_evict_set itsl)}):
+  (i:seq_index itsl{is_blum_evict itsl i /\ 
+                    blum_evict_elem itsl i = e})
+
+(* if the blum add occurs in the blum evict set, its index is earlier *)
+val lemma_evict_before_add (#p:pos) (itsl: its_log p) (i:seq_index itsl{is_blum_add (index itsl i)}):
+  Lemma (requires True)
+        (ensures (not (contains (blum_add_elem (index itsl i)) (ts_evict_set itsl)) \/
+                  index_blum_evict itsl (blum_add_elem (index itsl i)) < i))
+         
