Veritas.Verifier.Correctness.fst
@@ -14,6 +14,7 @@ open Veritas.State
 open Veritas.Verifier
 open Veritas.Verifier.CorrectDefs
 open Veritas.Verifier.EAC
+open Veritas.Verifier.TSLog
 
 //Allow the solver to unroll recursive functions at most once (fuel)
 //Allow the solver to invert inductive definitions at most once (ifuel)
@@ -30,7 +31,7 @@ let time_seq_idx (gl: g_hash_verifiable_log): its_log (length gl) =
 let to_state_op_gvlog (gl: g_vlog) =
   map to_state_op_vlog gl
 
-let lemma_time_seq_rw_consistent (#n:nat) 
+let lemma_time_seq_rw_consistent (#n:pos) 
   (itsl: its_log n{~ (rw_consistent (to_state_op_vlog (project_seq itsl)))}): hash_collision_gen = 
   let tsl = project_seq itsl in  
   let tsle = time_seq_ext itsl in
