Veritas.Verifier.TSLog.fst
@@ -1,0 +1,150 @@
+module Veritas.Verifier.TSLog
+
+let its_prefix_aux (#p:pos) (itsl: its_log p) (i:nat{i <= length itsl}): 
+  (itsl':its_log p{length itsl' = i}) =
+  let itsl': seq (idx_elem #vlog_entry p) = prefix itsl i in
+  let gl = partition_idx_seq itsl in
+  let idgl = g_tid_vlog gl in
+  
+  let gl' = partition_idx_seq itsl' in
+  let idgl' = g_tid_vlog gl' in
+
+  let aux (id:nat{id < p}):
+    Lemma (requires True)
+          (ensures (t_verifiable (index idgl' id)))
+          [SMTPat (t_verifiable (index idgl' id))]    
+    = 
+    let (_,l') = index idgl' id in
+    //let (_,l) = index idgl id in    
+    lemma_partition_idx_prefix_comm itsl i  id;
+    lemma_verifiable_implies_prefix_verifiable (index idgl id) (length l');
+    ()
+  in
+  itsl'
+
+let its_prefix (#p:pos) (itsl: its_log p) (i:nat{i <= length itsl}): 
+  (itsl':its_log p{itsl' = prefix itsl i}) = 
+  its_prefix_aux itsl i
+
+(* extended time sequence log (with evict values) *)
+let rec time_seq_ext_aux (#p:pos) (itsl: its_log p):
+  Tot (le:vlog_ext{project_seq itsl = to_vlog le})
+  (decreases (length itsl))
+  =
+  let m = length itsl in
+  if m = 0 then (
+    lemma_empty itsl;
+    lemma_empty (project_seq itsl);
+    let r = empty #vlog_entry_ext in
+    lemma_empty (to_vlog r);
+    r
+  )
+  else (
+    let (e,id) = telem itsl in
+
+    (* recurse *)
+    let itsl' = its_prefix itsl (m - 1) in
+    let r' = time_seq_ext_aux itsl' in
+
+    (* project seq of itsl and itsl' differ by log entry e *)
+    lemma_unzip_extend itsl;
+    assert(project_seq itsl = append1 (project_seq itsl') e);
+
+    if is_evict e then (
+      (* log entries of verifier thread id *)
+      let gl = partition_idx_seq itsl in
+      let l = index gl id in
+      assert(snd (index (g_tid_vlog gl) id) = l);
+
+      (* since l is verifiable, the value at last position is well-defined *)
+      assert(t_verifiable (id, l));
+      (* prove length l > 0 *)
+      lemma_partition_idx_extend1 itsl;
+
+      let v = evict_value (id, l) (length l - 1) in
+
+      let r = append1 r' (Evict e v) in
+      lemma_prefix1_append r' (Evict e v);
+      lemma_map_extend to_vlog_entry r;
+      r
+    )
+    else (
+      let r = append1 r' (NEvict e) in
+      lemma_prefix1_append r' (NEvict e);
+      lemma_map_extend to_vlog_entry r;
+      r
+    )
+  )
+
+let time_seq_ext = time_seq_ext_aux
+
+let lemma_its_prefix_ext (#n:pos) (itsl:its_log n) (i:nat{i <= length itsl}):
+  Lemma (requires True)
+        (ensures (time_seq_ext (its_prefix itsl i) = prefix (time_seq_ext itsl) i)) = 
+  admit()
+
+(* 
+ * when the eac state of a key is Init (no operations on the key yet) no 
+ * thread contains the key in its store 
+ *)
+let lemma_eac_state_init_store 
+   (#p:pos) 
+   (itsl: eac_ts_log p) (k: key{k <> Root && is_eac_state_init itsl k}) (id:nat{id < p}):
+   Lemma (not (store_contains (thread_store (verifier_thread_state itsl id)) k)) 
+   = admit()
+
+(* when the eac state of a key is EACEvicted then no thread contains the key in its store *)
+let lemma_eac_state_evicted_store (#p:pos) (itsl: eac_ts_log p) 
+  (k: key{is_eac_state_evicted itsl k}) (id:nat{id < p}):
+    Lemma (not (store_contains (thread_store (verifier_thread_state itsl id)) k)) = admit()
+
+(* when the eac state of a key is "instore" then there is always a previous add *)
+let lemma_eac_state_instore_implies_prev_add (#p:pos) (itsl: eac_ts_log p) (k:key{is_eac_state_instore itsl k}):
+  Lemma (has_some_add_of_key k (project_seq itsl)) = admit()
+
+(* if the eac_state of k is instore, then that k is in the store of the verifier thread of its last add *)
+let lemma_eac_state_instore (#p:pos) (itsl: eac_ts_log p) (k:key{is_eac_state_instore itsl k}):
+  Lemma (store_contains (thread_store (verifier_thread_state itsl (last_add_tid itsl k))) k) = admit()
+
+(* if the eac state of k is instore, then k is not in the store of any verifier thread other than 
+ * its last add thread *)
+let lemma_eac_state_instore2 (#p:pos) (itsl: eac_ts_log p) 
+  (k:key{is_eac_state_instore itsl k}) (id:nat{id < p}):
+  Lemma (requires (id <> last_add_tid itsl k))
+        (ensures (not (store_contains (thread_store (verifier_thread_state itsl id)) k))) = admit()
+
+(* the root is always in thread 0 *)
+let lemma_root_in_store0 (#p:pos) (itsl: eac_ts_log p):
+  Lemma (store_contains (thread_store (verifier_thread_state itsl 0)) Root) = admit()
+
+let lemma_root_not_in_store (#p:pos) (itsl: eac_ts_log p) (tid:pos {tid < p}):
+  Lemma (not (store_contains (thread_store (verifier_thread_state itsl tid)) Root)) = admit()
+
+(* the evicted value is always of the correct type for the associated key *)
+let lemma_evict_value_correct_type (#p:pos) (itsl: eac_ts_log p) (k:key{is_eac_state_evicted itsl k}):
+  Lemma (is_value_of k (EACEvicted?.v (eac_state_of_key itsl k))) = admit()
+
+
+(* 
+ * for keys in a thread store, return the value in the thread store; 
+ * for other keys return the last evict value or null (init)
+ *)
+let eac_value (#n:pos) (itsl: eac_ts_log n) (k:key): value_type_of k = 
+  if k = Root then (
+    lemma_root_in_store0 itsl;
+    stored_value (thread_store (verifier_thread_state itsl 0)) Root
+  )
+  else 
+    let es = eac_state_of_key itsl k in
+    match es with
+    | EACInit -> init_value k 
+    | EACEvicted _ v -> lemma_evict_value_correct_type itsl k; v
+    | EACInStore _ _ -> 
+      (* the store where the last add happened contains key k *)
+      let tid = last_add_tid itsl k in
+      let st = thread_store (verifier_thread_state itsl tid) in
+        
+      lemma_eac_state_instore itsl k;
+      assert(store_contains st k);
+
+      stored_value st k
