Veritas.Verifier.TSLog.fsti
@@ -1,0 +1,142 @@
+module Veritas.Verifier.TSLog
+
+open FStar.Seq
+open Veritas.BinTree
+open Veritas.EAC
+open Veritas.Interleave
+open Veritas.Key
+open Veritas.MultiSetHash
+open Veritas.Record
+open Veritas.SeqAux
+open Veritas.SeqMachine
+open Veritas.Verifier
+open Veritas.Verifier.CorrectDefs  
+
+type partition_verifiable (p:pos) (s: seq (idx_elem #vlog_entry p)) = 
+  g_verifiable (partition_idx_seq s)
+
+let clock (p:pos) (s: seq (idx_elem #vlog_entry p){partition_verifiable p s}) (i: seq_index s): 
+  timestamp = 
+  let gl = partition_idx_seq s in
+  admit()
+
+type clock_sorted (p:pos) (s: seq (idx_elem #vlog_entry p){partition_verifiable p s}) =
+  forall (i:seq_index s). i > 0 ==> clock p s (i - 1) `ts_leq` clock p s i
+
+type its_log (p:pos) = 
+  s:seq (idx_elem #vlog_entry p){partition_verifiable p s /\ clock_sorted p s}
+
+(* prefix of an its log *)
+val its_prefix (#p:pos) (itsl: its_log p) (i:nat{i <= length itsl}): 
+  (itsl':its_log p{itsl' = prefix itsl i})
+
+(* extended time sequence log (with evict values) *)
+val time_seq_ext (#p:pos) (itsl: its_log p):
+  Tot (le:vlog_ext{project_seq itsl = to_vlog le})
+
+val lemma_its_prefix_ext (#n:pos) (itsl:its_log n) (i:nat{i <= length itsl}):
+  Lemma (requires True)
+        (ensures (time_seq_ext (its_prefix itsl i) = prefix (time_seq_ext itsl) i))
+        [SMTPat (time_seq_ext (its_prefix itsl i))]
+  
+type eac_ts_log (p:pos) = itsl: its_log p {is_eac_log (time_seq_ext itsl)}
+type non_eac_ts_log (p:pos) = itsl: its_log p {not (is_eac_log (time_seq_ext itsl))}
+
+(* the eac state of a key at the end of an its log *)
+let eac_state_of_key (#p:pos) (itsl: its_log p) (k:key): eac_state = 
+  let tsle = time_seq_ext itsl in 
+  let tslek = partn eac_sm k tsle in
+  seq_machine_run eac_smk tslek
+
+(* is the eac state of key at the end of its_log init *)
+let is_eac_state_init (#p:pos) (itsl: its_log p) (k:key): bool =
+  eac_state_of_key itsl k = EACInit
+
+(* is the key k in evicted state in *)
+let is_eac_state_evicted (#p:pos) (itsl: its_log p) (k:key): bool = 
+  EACEvicted? (eac_state_of_key itsl k)
+
+(* is the key currently evicted into merkle *)
+let is_eac_state_evicted_merkle (#p:pos) (itsl: its_log p) (k:key): bool = 
+  let st = eac_state_of_key itsl k in
+  match st with
+  | EACEvicted m v -> m = MAdd 
+  | _ -> false
+
+(* is the key currently evicted into merkle *)
+let is_eac_state_evicted_blum (#p:pos) (itsl: its_log p) (k:key): bool = 
+  let st = eac_state_of_key itsl k in
+  match st with
+  | EACEvicted m v -> m = BAdd
+  | _ -> false
+
+(* is the key k in instore state after processing its_log *)
+let is_eac_state_instore (#p:pos) (itsl: its_log p) (k:key):bool = 
+  EACInStore? (eac_state_of_key itsl k)
+
+(* the state of a verifier thread after processing entries in a log *)
+let verifier_thread_state (#p:pos) (itsl: its_log p) (id:nat{id < p}): (st:vtls{Valid? st}) = 
+  let gl = partition_idx_seq itsl in
+  assert(t_verifiable (index (attach_index gl) id));
+  t_verify id (index gl id)
+
+(* 
+ * when the eac state of a key is Init (no operations on the key yet) no 
+ * thread contains the key in its store 
+ *)
+val lemma_eac_state_init_store 
+   (#p:pos) 
+   (itsl: eac_ts_log p) (k: key{k <> Root && is_eac_state_init itsl k}) (id:nat{id < p}):
+   Lemma (not (store_contains (thread_store (verifier_thread_state itsl id)) k)) 
+
+(* when the eac state of a key is EACEvicted then no thread contains the key in its store *)
+val lemma_eac_state_evicted_store (#p:pos) (itsl: eac_ts_log p) 
+  (k: key{is_eac_state_evicted itsl k}) (id:nat{id < p}):
+  Lemma (not (store_contains (thread_store (verifier_thread_state itsl id)) k))
+  
+(* when the eac state of a key is "instore" then there is always a previous add *)
+val lemma_eac_state_instore_implies_prev_add (#p:pos) (itsl: eac_ts_log p) 
+  (k:key{is_eac_state_instore itsl k}):
+  Lemma (has_some_add_of_key k (project_seq itsl))
+
+(* when the eac state of a key is instore return the index of the last add that transitioned
+ * the key k to "instore" *)
+let last_add_idx (#p:pos) (itsl: eac_ts_log p) (k: key{is_eac_state_instore itsl k}): seq_index itsl =
+   lemma_eac_state_instore_implies_prev_add itsl k;
+   last_index (is_add_of_key k) (project_seq itsl)
+
+(* the verifier thread where the last add of key k happens *)
+let last_add_tid (#p:pos) (itsl: eac_ts_log p) (k: key{is_eac_state_instore itsl k}): (tid:nat{tid < p}) =
+  snd (index itsl (last_add_idx itsl k))
+
+(* if the eac_state of k is instore, then that k is in the store of the verifier thread of its last add *)
+val lemma_eac_state_instore (#p:pos) (itsl: eac_ts_log p) (k:key{is_eac_state_instore itsl k}):
+  Lemma (store_contains (thread_store (verifier_thread_state itsl (last_add_tid itsl k))) k)
+
+(* if the eac state of k is instore, then k is not in the store of any verifier thread other than 
+ * its last add thread *)
+val lemma_eac_state_instore2 (#p:pos) (itsl: eac_ts_log p) 
+  (k:key{is_eac_state_instore itsl k}) (id:nat{id < p}):
+  Lemma (requires (id <> last_add_tid itsl k))
+        (ensures (not (store_contains (thread_store (verifier_thread_state itsl id)) k)))
+
+(* the root is always in thread 0 *)
+val lemma_root_in_store0 (#p:pos) (itsl: eac_ts_log p):
+  Lemma (store_contains (thread_store (verifier_thread_state itsl 0)) Root)
+
+val lemma_root_not_in_store (#p:pos) (itsl: eac_ts_log p) (tid:pos {tid < p}):
+  Lemma (not (store_contains (thread_store (verifier_thread_state itsl tid)) Root))
+
+(* the evicted value is always of the correct type for the associated key *)
+val lemma_evict_value_correct_type (#p:pos) (itsl: eac_ts_log p) (k:key{is_eac_state_evicted itsl k}):
+  Lemma (is_value_of k (EACEvicted?.v (eac_state_of_key itsl k)))
+
+(* 
+ * for keys in a thread store, return the value in the thread store; 
+ * for other keys return the last evict value or null (init)
+ *)
+ val eac_value (#n:pos) (itsl: eac_ts_log n) (k:key): value_type_of k
+
+let key_of (#p:pos) (itsl: its_log p) (i: seq_index itsl): key = 
+  let (e,_) = index itsl i in
+  vlog_entry_key e
